Created state theorems file

States.v
@@ -59,99 +59,16 @@ Definition state_pred_inductive
   {Scalar} {State}
   {sops : ScalarOps Scalar}
   {state_ops : StateOps Scalar State}
-  (B : Ensemble State) (P : State -> Prop) : Prop :=
-  (forall (S : State), In State B S -> P S) /\
+  (P : State -> Prop) : Prop :=
   (forall (S1 S2 : State), P S1 -> P S2 -> P (join S1 S2)) /\
   (forall (S1 S2 : State), P S1 -> P S2 -> P (meet S1 S2)) /\
   (forall (S : State) (a : Scalar), P S -> P (scalar_prod a S)) /\
   (forall (S : State), P S -> P (~ S)) /\
   P null.
 
-(* Helper used in proof of the induction principle over a basis. *)
-Definition P_if_basis
+Definition state_pred_forall_basis
   {Scalar} {State}
   {sops : ScalarOps Scalar}
   {state_ops : StateOps Scalar State}
-  (P : State -> Prop) (B : Ensemble State) (S : State) :=
-  state_basis B S -> P S.
-
-(* Induction theorem with basis sets.  Any inductive predicate P over
- * a basis B holds for all elements of any state S such that B is a
- * basis for S.
- *)
-Theorem state_basis_induction
-  {Scalar} {State}
-  {sops : ScalarOps Scalar}
-  {state_ops : StateOps Scalar State}
-  (B : Ensemble State) (P : State -> Prop) :
-  state_pred_inductive B P -> (forall (S : State), state_basis B S -> P S).
-Proof.
-  unfold state_pred_inductive.
-  intros (basis_P & join_P & meet_P & scalar_P & conj_P & null_P).
-  intros.
-  cut (state_basis B S).
-  revert H.
-  replace (state_basis B S -> P S) with (P_if_basis P B S).
-  apply (state_basis_ind Scalar State sops state_ops B).
-  unfold P_if_basis.
-  intro.
-  assumption.
-  intros.
-  unfold P_if_basis.
-  intro.
-  apply basis_P.
-  assumption.
-  unfold P_if_basis.
-  intros.
-  apply join_P.
-  apply H0.
-  assumption.
-  apply H2.
-  assumption.
-  unfold P_if_basis.
-  intros.
-  apply meet_P.
-  apply H0.
-  assumption.
-  apply H2.
-  assumption.
-  unfold P_if_basis.
-  intros.
-  apply scalar_P.
-  apply H0.
-  assumption.
-  unfold P_if_basis.
-  intros.
-  apply conj_P.
-  apply H0.
-  assumption.
-  unfold P_if_basis.
-  reflexivity.
-  assumption.
-Qed.
-
-(* Is B a basis for all states in set SS? *)
-Definition state_set_basis
-  {Scalar} {State}
-  {sops : ScalarOps Scalar}
-  {state_ops : StateOps Scalar State}
-  (B : Ensemble State) (SS : Ensemble State) :=
-  forall (S : State), In State SS S -> state_basis B S.
-
-(* A version of the basis induction theorem for sets of states. *)
-Lemma state_set_basis_induction
-  {Scalar} {State}
-  {sops : ScalarOps Scalar}
-  {state_ops : StateOps Scalar State}
-  (B : Ensemble State) (SS : Ensemble State) (P : State -> Prop) :
-  state_pred_inductive B P -> state_set_basis B SS ->
-  (forall (S : State), In State SS S -> P S).
-Proof.
-  intro.
-  unfold state_set_basis.
-  intros.
-  apply H0 in H1.
-  apply (state_basis_induction B).
-  assumption.
-  assumption.
-Qed.
+  (B : Ensemble State) (P : State -> Prop) : Prop :=
+  forall (S : State), In State B S -> P S.
