StateTheorems.v
@@ -1,0 +1,97 @@
+Require Import New.Complex.
+Require Import New.Field.
+Require Import Scalars.
+Require Import States.
+Require Import Coq.Sets.Ensembles.
+
+(* Helper used in proof of the induction principle over a basis. *)
+Definition P_if_basis
+  {Scalar} {State}
+  {sops : ScalarOps Scalar}
+  {state_ops : StateOps Scalar State}
+  (P : State -> Prop) (B : Ensemble State) (S : State) :=
+  state_basis B S -> P S.
+
+(* Induction theorem with basis sets.  Any inductive predicate P over
+ * a basis B holds for all elements of any state S such that B is a
+ * basis for S.
+ *)
+Theorem state_basis_induction
+  {Scalar} {State}
+  {sops : ScalarOps Scalar}
+  {state_ops : StateOps Scalar State}
+  (B : Ensemble State) (P : State -> Prop) :
+  state_pred_inductive P -> state_pred_forall_basis B P ->
+  (forall (S : State), state_basis B S -> P S).
+Proof.
+  unfold state_pred_inductive.
+  intros (join_P & meet_P & scalar_P & conj_P & null_P).
+  unfold state_pred_forall_basis.
+  intro basis_P.
+  intros.
+  cut (state_basis B S).
+  revert H.
+  replace (state_basis B S -> P S) with (P_if_basis P B S).
+  apply (state_basis_ind Scalar State sops state_ops B).
+  unfold P_if_basis.
+  intro.
+  assumption.
+  intros.
+  unfold P_if_basis.
+  intro.
+  apply basis_P.
+  assumption.
+  unfold P_if_basis.
+  intros.
+  apply join_P.
+  apply H0.
+  assumption.
+  apply H2.
+  assumption.
+  unfold P_if_basis.
+  intros.
+  apply meet_P.
+  apply H0.
+  assumption.
+  apply H2.
+  assumption.
+  unfold P_if_basis.
+  intros.
+  apply scalar_P.
+  apply H0.
+  assumption.
+  unfold P_if_basis.
+  intros.
+  apply conj_P.
+  apply H0.
+  assumption.
+  unfold P_if_basis.
+  reflexivity.
+  assumption.
+Qed.
+
+(* Is B a basis for all states in set SS? *)
+Definition state_set_basis
+  {Scalar} {State}
+  {sops : ScalarOps Scalar}
+  {state_ops : StateOps Scalar State}
+  (B : Ensemble State) (SS : Ensemble State) :=
+  forall (S : State), In State SS S -> state_basis B S.
+
+(* A version of the basis induction theorem for sets of states. *)
+Lemma state_set_basis_induction
+  {Scalar} {State}
+  {sops : ScalarOps Scalar}
+  {state_ops : StateOps Scalar State}
+  (B : Ensemble State) (SS : Ensemble State) (P : State -> Prop) :
+  state_pred_inductive P -> state_pred_forall_basis B P ->
+  state_set_basis B SS -> (forall (S : State), In State SS S -> P S).
+Proof.
+  unfold state_set_basis.
+  intros.
+  apply H1 in H2.
+  apply (state_basis_induction B).
+  assumption.
+  assumption.
+  assumption.
+Qed.
